
\begin{document}
\[
x(t) = \sum\limits_{n =  - \infty }^\infty  {a_n } g(t - nT)
\]

\[
\begin{array}{l}
 \sum\limits_{i = 0}^N i  = \frac{{N(N + 1)}}{2}:\sqrt[3]{{27}} = 3 \\ 
 \sqrt[3]{{45}} \\ 
 \end{array}
\]
\[
S_x (f) = f_n \left| {P(f)} \right|^2 \{ X_c (f) + f_n X_d (f)\sum\limits_{i =  - \infty }^\infty  \delta  (f - if_n )\} 
\]
\[
\begin{array}{l}
 {\bf{R}}_m  = {\bf{E}}\{ {\bf{c}}_{\bf{i}} {\bf{c}}_{{\bf{i}} + {\bf{m}}} \}  \\ 
  \\ 
 \end{array}
\]
\[
\begin{array}{l}
 {\bf{R}}_m  = {\bf{A}}^{\bf{T}} {\bf{P}}_{\bf{m}} {\bf{A}} \\ 
  \\ 
 \end{array}
\]\[
X_c (f) = v\Gamma _1 v* + 2\Re \{ {\bf{v}}\Gamma _2 {\bf{v}}^* \} 
\]
\[
R_\infty   = \mathop {\lim }\limits_{k \to \infty } {\bf{R}}_{\bf{k}} 
\]
\[
X_d (f) = {\bf{vR}}_\infty  {\bf{v}}^* 
\]
\[
{\bf{v}} = [{\bf{e}}^{{\bf{j}}\omega {\bf{T}}_{\bf{b}} } ,{\bf{e}}^{{\bf{j}}\omega 2{\bf{T}}_{\bf{b}} } ,{\bf{e}}^{{\bf{j}}\omega 3{\bf{T}}_{\bf{b}} } , \ldots ,{\bf{e}}^{{\bf{j}}\omega n{\bf{T}}_{\bf{b}} } ]
\]
\[
{\bf{v}} = [{\bf{e}}^{ - {\bf{j}}\omega {\bf{T}}_{\bf{b}} } ,{\bf{e}}^{ - {\bf{j}}\omega 2{\bf{T}}_{\bf{b}} } ,{\bf{e}}^{ - {\bf{j}}\omega 3{\bf{T}}_{\bf{b}} } , \ldots ,{\bf{e}}^{ - {\bf{j}}\omega n{\bf{T}}_{\bf{b}} } ]
\]
\[
\Gamma _{\bf{1}}  = {\bf{R}}_{\bf{0}}  - {\bf{R}}_\infty  
\]
\[
\Gamma _{\bf{2}}  = \sum\limits_{{\bf{k}} = {\bf{1}}}^\infty  {{\bf{e}}^{ - {\bf{j}}\omega {\bf{kT}}_{\bf{n}} } } ({\bf{R}}_{\bf{k}}  - {\bf{R}}_\infty  ) = 0
\]

\[
X_c (f) = vA^T (\frac{1}{k}I - \frac{1}{{k^2 }}U)Av^* 
\]

\[
X_d (f) = \frac{1}{{k^2 }}vA^T UAv^* 
\]

\[
R_0  = \frac{1}{k}A^T IA
\]

\[
R_k  = R_\infty   = \frac{1}{{k^2 }}A^T UA
\]

\[

\]

\[
U = \left[ \begin{array}{l}
 1 & 1 &  \cdots  & 1 \\ 
 1 & 1 &  \cdots  & 1 \\ 
  \vdots  &  \vdots  &  \cdots  &  \vdots  \\ 
 1 & 1 &  \cdots  & 1 \\ 
 \end{array} \right]
\]

\end{document}